@prefix : <http://www.EcoInvent.org/EcoSpold02/flowdata#> .
@prefix j.0: <http://www.EcoInvent.org/EcoSpold02#> .
@prefix j.1: <http://www.w3.org/XML/1998/namespace#> .
@prefix owl: <http://www.w3.org/2002/07/owl#> .
@prefix rdf: <http://www.w3.org/1999/02/22-rdf-syntax-ns#> .
@prefix xml: <http://www.w3.org/XML/1998/namespace> .
@prefix xsd: <http://www.w3.org/2001/XMLSchema#> .
@prefix rdfs: <http://www.w3.org/2000/01/rdf-schema#> .
@prefix dtype: <http://www.srdc.com.tr/ontmalizer#> .
@base <http://www.EcoInvent.org/EcoSpold02/flowdata> .

<http://www.EcoInvent.org/EcoSpold02/flowdata> rdf:type owl:Ontology .

#################################################################
#    Annotation properties
#################################################################

###  http://www.srdc.com.tr/ontmalizer#hasValue
dtype:hasValue rdf:type owl:AnnotationProperty .


###  http://www.w3.org/2001/XMLSchema#length
xsd:length rdf:type owl:AnnotationProperty .


###  http://www.w3.org/2001/XMLSchema#maxInclusive
xsd:maxInclusive rdf:type owl:AnnotationProperty .


###  http://www.w3.org/2001/XMLSchema#maxLength
xsd:maxLength rdf:type owl:AnnotationProperty .


###  http://www.w3.org/2001/XMLSchema#minInclusive
xsd:minInclusive rdf:type owl:AnnotationProperty .


###  http://www.w3.org/2001/XMLSchema#pattern
xsd:pattern rdf:type owl:AnnotationProperty .


###  http://www.w3.org/2002/07/owl#maxCardinality
owl:maxCardinality rdf:type owl:AnnotationProperty .


#################################################################
#    Datatypes
#################################################################

###  http://www.w3.org/2001/XMLSchema#ENTITIESDatatype
xsd:ENTITIESDatatype rdf:type rdfs:Datatype .


###  http://www.w3.org/2001/XMLSchema#ENTITYDatatype
xsd:ENTITYDatatype rdf:type rdfs:Datatype .


###  http://www.w3.org/2001/XMLSchema#IDDatatype
xsd:IDDatatype rdf:type rdfs:Datatype .


###  http://www.w3.org/2001/XMLSchema#IDREFDatatype
xsd:IDREFDatatype rdf:type rdfs:Datatype .


###  http://www.w3.org/2001/XMLSchema#IDREFSDatatype
xsd:IDREFSDatatype rdf:type rdfs:Datatype .


###  http://www.w3.org/2001/XMLSchema#NCNameDatatype
xsd:NCNameDatatype rdf:type rdfs:Datatype .


###  http://www.w3.org/2001/XMLSchema#NMTOKENDatatype
xsd:NMTOKENDatatype rdf:type rdfs:Datatype .


###  http://www.w3.org/2001/XMLSchema#NMTOKENSDatatype
xsd:NMTOKENSDatatype rdf:type rdfs:Datatype .


###  http://www.w3.org/2001/XMLSchema#NOTATIONDatatype
xsd:NOTATIONDatatype rdf:type rdfs:Datatype .


###  http://www.w3.org/2001/XMLSchema#NameDatatype
xsd:NameDatatype rdf:type rdfs:Datatype .


###  http://www.w3.org/2001/XMLSchema#QNameDatatype
xsd:QNameDatatype rdf:type rdfs:Datatype .


###  http://www.w3.org/2001/XMLSchema#anySimpleTypeDatatype
xsd:anySimpleTypeDatatype rdf:type rdfs:Datatype .


###  http://www.w3.org/2001/XMLSchema#anyURIDatatype
xsd:anyURIDatatype rdf:type rdfs:Datatype .


###  http://www.w3.org/2001/XMLSchema#base64BinaryDatatype
xsd:base64BinaryDatatype rdf:type rdfs:Datatype .


###  http://www.w3.org/2001/XMLSchema#booleanDatatype
xsd:booleanDatatype rdf:type rdfs:Datatype .


###  http://www.w3.org/2001/XMLSchema#byteDatatype
xsd:byteDatatype rdf:type rdfs:Datatype .


###  http://www.w3.org/2001/XMLSchema#dateDatatype
xsd:dateDatatype rdf:type rdfs:Datatype .


###  http://www.w3.org/2001/XMLSchema#dateTimeDatatype
xsd:dateTimeDatatype rdf:type rdfs:Datatype .


###  http://www.w3.org/2001/XMLSchema#decimalDatatype
xsd:decimalDatatype rdf:type rdfs:Datatype .


###  http://www.w3.org/2001/XMLSchema#doubleDatatype
xsd:doubleDatatype rdf:type rdfs:Datatype .


###  http://www.w3.org/2001/XMLSchema#durationDatatype
xsd:durationDatatype rdf:type rdfs:Datatype .


###  http://www.w3.org/2001/XMLSchema#floatDatatype
xsd:floatDatatype rdf:type rdfs:Datatype .


###  http://www.w3.org/2001/XMLSchema#gDayDatatype
xsd:gDayDatatype rdf:type rdfs:Datatype .


###  http://www.w3.org/2001/XMLSchema#gMonthDatatype
xsd:gMonthDatatype rdf:type rdfs:Datatype .


###  http://www.w3.org/2001/XMLSchema#gMonthDayDatatype
xsd:gMonthDayDatatype rdf:type rdfs:Datatype .


###  http://www.w3.org/2001/XMLSchema#gYearDatatype
xsd:gYearDatatype rdf:type rdfs:Datatype .


###  http://www.w3.org/2001/XMLSchema#gYearMonthDatatype
xsd:gYearMonthDatatype rdf:type rdfs:Datatype .


###  http://www.w3.org/2001/XMLSchema#hexBinaryDatatype
xsd:hexBinaryDatatype rdf:type rdfs:Datatype .


###  http://www.w3.org/2001/XMLSchema#intDatatype
xsd:intDatatype rdf:type rdfs:Datatype .


###  http://www.w3.org/2001/XMLSchema#integerDatatype
xsd:integerDatatype rdf:type rdfs:Datatype .


###  http://www.w3.org/2001/XMLSchema#languageDatatype
xsd:languageDatatype rdf:type rdfs:Datatype .


###  http://www.w3.org/2001/XMLSchema#longDatatype
xsd:longDatatype rdf:type rdfs:Datatype .


###  http://www.w3.org/2001/XMLSchema#negativeIntegerDatatype
xsd:negativeIntegerDatatype rdf:type rdfs:Datatype .


###  http://www.w3.org/2001/XMLSchema#nonNegativeIntegerDatatype
xsd:nonNegativeIntegerDatatype rdf:type rdfs:Datatype .


###  http://www.w3.org/2001/XMLSchema#nonPositiveIntegerDatatype
xsd:nonPositiveIntegerDatatype rdf:type rdfs:Datatype .


###  http://www.w3.org/2001/XMLSchema#normalizedStringDatatype
xsd:normalizedStringDatatype rdf:type rdfs:Datatype .


###  http://www.w3.org/2001/XMLSchema#positiveIntegerDatatype
xsd:positiveIntegerDatatype rdf:type rdfs:Datatype .


###  http://www.w3.org/2001/XMLSchema#shortDatatype
xsd:shortDatatype rdf:type rdfs:Datatype .


###  http://www.w3.org/2001/XMLSchema#stringDatatype
xsd:stringDatatype rdf:type rdfs:Datatype .


###  http://www.w3.org/2001/XMLSchema#timeDatatype
xsd:timeDatatype rdf:type rdfs:Datatype .


###  http://www.w3.org/2001/XMLSchema#tokenDatatype
xsd:tokenDatatype rdf:type rdfs:Datatype .


###  http://www.w3.org/2001/XMLSchema#unsignedByteDatatype
xsd:unsignedByteDatatype rdf:type rdfs:Datatype .


###  http://www.w3.org/2001/XMLSchema#unsignedIntDatatype
xsd:unsignedIntDatatype rdf:type rdfs:Datatype .


###  http://www.w3.org/2001/XMLSchema#unsignedLongDatatype
xsd:unsignedLongDatatype rdf:type rdfs:Datatype .


###  http://www.w3.org/2001/XMLSchema#unsignedShortDatatype
xsd:unsignedShortDatatype rdf:type rdfs:Datatype .


#################################################################
#    Object Properties
#################################################################

###  http://www.EcoInvent.org/EcoSpold02/flowdata#compartment
:compartment rdf:type owl:ObjectProperty ;
             rdfs:domain :TElementaryExchange ;
             rdfs:comment "Name of the compartment and subcompartment of the exchange. The xml document referenced by validCompartments contains definitions of valid compartment/subcompartment pairs for a given language." .


###  http://www.EcoInvent.org/EcoSpold02/flowdata#inputGroup
:inputGroup rdf:type owl:ObjectProperty ;
            rdfs:domain :TIntermediateExchange ;
            rdfs:comment """Indicates the kind of input flow. 
The codes are: 1=Materials/Fuels, 2=Electricity/Heat, 3=Services, 5=From Technosphere (unspecified).
						For each exchange only an inputGroup or outputGroup shall exist. This indicates the direction of the flow.""" .


###  http://www.EcoInvent.org/EcoSpold02/flowdata#outputGroup
:outputGroup rdf:type owl:ObjectProperty ;
             rdfs:domain :TIntermediateExchange ;
             rdfs:comment """Indicates the kind of output flow. 
The codes are: 0=ReferenceProduct, 2=By-product, 3=MaterialForTreatment, 5=Stock Additions
For each exchange only an inputGroup or outputGroup shall exist. This indicates the direction of the flow.""" .


###  http://www.EcoInvent.org/EcoSpold02/flowdata#productionVolumeUncertainty
:productionVolumeUncertainty rdf:type owl:ObjectProperty ;
                             rdfs:domain :TCustomExchange ;
                             rdfs:comment """Uncertainty information in the form of distribution functions and their parameters and/or pedigree data.
						For the format definition see the complex type section below.""" .


###  http://www.EcoInvent.org/EcoSpold02/flowdata#property
:property rdf:type owl:ObjectProperty ;
          rdfs:domain :TCustomExchange ;
          rdfs:comment """Properties of the exchange, e.g. dry mass, water content, price, content of specific elements or substances.

For the format definition see the complex type section below.""" .


###  http://www.EcoInvent.org/EcoSpold02/flowdata#transferCoefficient
:transferCoefficient rdf:type owl:ObjectProperty ;
                     rdfs:domain :TCustomExchange ;
                     rdfs:range :TTransferCoefficient ;
                     rdfs:comment """Transfer coefficients relate specific inputs to specific outputs and record the share of this specific input that contributes to this specific output.

For the  format definition see the complex  type section below.""" .


#################################################################
#    Data properties
#################################################################

###  http://www.EcoInvent.org/EcoSpold02/flowdata#activityLinkContextId
:activityLinkContextId rdf:type owl:DatatypeProperty ;
                       rdfs:domain :TIntermediateExchange ;
                       rdfs:range xsd:string ;
                       rdfs:comment """Reference to the context of the activity link.

If this attribute is omitted the context of the dataset itself will be used instead.""" .


###  http://www.EcoInvent.org/EcoSpold02/flowdata#activityLinkId
:activityLinkId rdf:type owl:DatatypeProperty ;
                rdfs:domain :TIntermediateExchange ;
                rdfs:range xsd:string ;
                rdfs:comment "Explicit reference to the activity which supplies the intermediate product. If this field is empty the activity will determined by a linking rule, which uses geographical and temporal information of this activity." .


###  http://www.EcoInvent.org/EcoSpold02/flowdata#activityLinkIdOverwrittenByChild
:activityLinkIdOverwrittenByChild rdf:type owl:DatatypeProperty ;
                                  rdfs:domain :TIntermediateExchange ;
                                  rdfs:range xsd:string ;
                                  rdfs:comment "If a reference to a master data entity must be removed in a child dataset it is required to set the corresponding xxxOverwrittenByChild attribute to true. Otherwise the removed referenced will be interpreted as \"Keep the Parent Value\"." .


###  http://www.EcoInvent.org/EcoSpold02/flowdata#amount
:amount rdf:type owl:DatatypeProperty ;
        rdfs:domain :TElementaryExchange ,
                    :TIntermediateExchange ,
                    :TParameter ,
                    :TTransferCoefficient ;
        rdfs:range xsd:float ;
        rdfs:comment "Amount of an elementary or intermediate exchange." .


###  http://www.EcoInvent.org/EcoSpold02/flowdata#casNumber
:casNumber rdf:type owl:DatatypeProperty ;
           rdfs:domain :TElementaryExchange ;
           rdfs:range xsd:string ;
           rdfs:comment "Indicates the number according to the Chemical Abstract Service (CAS). The Format of the CAS-number: 000000-00-0, where the first string of digits needs not to be complete (i.e. less than six digits are admitted)." .


###  http://www.EcoInvent.org/EcoSpold02/flowdata#elementaryExchangeContextId
:elementaryExchangeContextId rdf:type owl:DatatypeProperty ;
                             rdfs:domain :TElementaryExchange ;
                             rdfs:range xsd:string ;
                             rdfs:comment """Reference to the context of the elementary exchange.
						If this attribute is omitted the context of the dataset itself will be used instead.""" .


###  http://www.EcoInvent.org/EcoSpold02/flowdata#elementaryExchangeId
:elementaryExchangeId rdf:type owl:DatatypeProperty ;
                      rdfs:domain :TElementaryExchange ;
                      rdfs:range xsd:string ;
                      rdfs:comment "Reference to the master data entry for this elementary exchange" .


###  http://www.EcoInvent.org/EcoSpold02/flowdata#exchangeId
:exchangeId rdf:type owl:DatatypeProperty ;
            rdfs:domain :TElementaryExchange ,
                        :TTransferCoefficient ;
            rdfs:range xsd:string ;
            rdfs:comment "Reference to the UUID of an exchange." .


###  http://www.EcoInvent.org/EcoSpold02/flowdata#formula
:formula rdf:type owl:DatatypeProperty ;
         rdfs:domain :TElementaryExchange ;
         rdfs:range xsd:string ;
         rdfs:comment "Chemical formula (e.g. sum formula) may be entered." .


###  http://www.EcoInvent.org/EcoSpold02/flowdata#impactCategoryContextId
:impactCategoryContextId rdf:type owl:DatatypeProperty ;
                         rdfs:domain :TImpactIndicatorResult ;
                         rdfs:range xsd:string ;
                         rdfs:comment "Reference to the context of the impact category. If this attribute is omitted the context of the dataset itself will be used instead." .


###  http://www.EcoInvent.org/EcoSpold02/flowdata#impactCategoryId
:impactCategoryId rdf:type owl:DatatypeProperty ;
                  rdfs:domain :TImpactIndicatorResult ;
                  rdfs:range xsd:string ;
                  rdfs:comment "Reference to the method of the impact category." .


###  http://www.EcoInvent.org/EcoSpold02/flowdata#impactCategoryName
:impactCategoryName rdf:type owl:DatatypeProperty ;
                    rdfs:domain :TImpactIndicatorResult ;
                    rdfs:range xsd:string ;
                    rdfs:comment "Name of the impact category." .


###  http://www.EcoInvent.org/EcoSpold02/flowdata#impactIndicatorContextId
:impactIndicatorContextId rdf:type owl:DatatypeProperty ;
                          rdfs:domain :TImpactIndicatorResult ;
                          rdfs:range xsd:string ;
                          rdfs:comment "Reference to the context of the impact indicator. If this attribute is omitted the context of the dataset itself will be used instead." .


###  http://www.EcoInvent.org/EcoSpold02/flowdata#impactIndicatorId
:impactIndicatorId rdf:type owl:DatatypeProperty ;
                   rdfs:domain :TImpactIndicatorResult ;
                   rdfs:range xsd:string ;
                   rdfs:comment "Reference to the impact indicator." .


###  http://www.EcoInvent.org/EcoSpold02/flowdata#impactMethodContextId
:impactMethodContextId rdf:type owl:DatatypeProperty ;
                       rdfs:domain :TImpactIndicatorResult ;
                       rdfs:range xsd:string ;
                       rdfs:comment "Reference to the context of the impact method. If this attribute is omitted the context of the dataset itself will be used instead." .


###  http://www.EcoInvent.org/EcoSpold02/flowdata#impactMethodId
:impactMethodId rdf:type owl:DatatypeProperty ;
                rdfs:domain :TImpactIndicatorResult ;
                rdfs:range xsd:string ;
                rdfs:comment "Reference to the method of the impact indicator." .


###  http://www.EcoInvent.org/EcoSpold02/flowdata#impactMethodName
:impactMethodName rdf:type owl:DatatypeProperty ;
                  rdfs:domain :TImpactIndicatorResult ;
                  rdfs:range xsd:string ;
                  rdfs:comment "Name of the impact method." .


###  http://www.EcoInvent.org/EcoSpold02/flowdata#intermediateExchangeContextId
:intermediateExchangeContextId rdf:type owl:DatatypeProperty ;
                               rdfs:domain :TIntermediateExchange ;
                               rdfs:range xsd:string ;
                               rdfs:comment """Reference to the context of the intermediate exchange.

If this attribute is omitted the context of the dataset itself will be used instead.""" .


###  http://www.EcoInvent.org/EcoSpold02/flowdata#intermediateExchangeId
:intermediateExchangeId rdf:type owl:DatatypeProperty ;
                        rdfs:domain :TIntermediateExchange ;
                        rdfs:range xsd:string ;
                        rdfs:comment "Reference to the master data entry for this intermediate exchange" .


###  http://www.EcoInvent.org/EcoSpold02/flowdata#isCalculatedAmount
:isCalculatedAmount rdf:type owl:DatatypeProperty ;
                    rdfs:domain :TElementaryExchange ,
                                :TParameter ,
                                :TTransferCoefficient ;
                    rdfs:range xsd:boolean ;
                    rdfs:comment "If true the value of the amount field is the calculated value of the mathematicalRelation or the transferCoefficient." .


###  http://www.EcoInvent.org/EcoSpold02/flowdata#mathematicalRelation
:mathematicalRelation rdf:type owl:DatatypeProperty ;
                      rdfs:domain :TElementaryExchange ,
                                  :TParameter ,
                                  :TTransferCoefficient ;
                      rdfs:range xsd:string ;
                      rdfs:comment """Defines a mathematical formula with references to values of flows, parameters or properties by variable names or REF function.
The result of the formula with a specific set of variable values is written into the amount field.""" .


###  http://www.EcoInvent.org/EcoSpold02/flowdata#name
:name rdf:type owl:DatatypeProperty ;
      rdfs:domain :TCustomExchange ,
                  :TElementaryExchange ,
                  :TImpactIndicatorResult ,
                  :TParameter ;
      rdfs:range xsd:string ;
      rdfs:comment "Name of the exchange/parameter" .


###  http://www.EcoInvent.org/EcoSpold02/flowdata#pageNumbers
:pageNumbers rdf:type owl:DatatypeProperty ;
             rdfs:domain :TElementaryExchange ;
             rdfs:range xsd:string ;
             rdfs:comment "The relevant page numbers if the data are sourced on specific pages in an article or larger publication." .


###  http://www.EcoInvent.org/EcoSpold02/flowdata#parameterContextId
:parameterContextId rdf:type owl:DatatypeProperty ;
                    rdfs:domain :TParameter ;
                    rdfs:range xsd:string ;
                    rdfs:comment """Reference to the context of the parameter.

If this attribute is omitted the context of the dataset itself will be used instead.""" .


###  http://www.EcoInvent.org/EcoSpold02/flowdata#parameterId
:parameterId rdf:type owl:DatatypeProperty ;
             rdfs:domain :TParameter ;
             rdfs:range xsd:string ;
             rdfs:comment "A reference to a valid master data parameter." .


###  http://www.EcoInvent.org/EcoSpold02/flowdata#productionVolumeAmount
:productionVolumeAmount rdf:type owl:DatatypeProperty ;
                        rdfs:domain :TIntermediateExchange ;
                        rdfs:range xsd:float ;
                        rdfs:comment "The product volume expressed per year in the same unit as the exchange." .


###  http://www.EcoInvent.org/EcoSpold02/flowdata#productionVolumeComment
:productionVolumeComment rdf:type owl:DatatypeProperty ;
                         rdfs:domain :TIntermediateExchange ;
                         rdfs:range xsd:string ;
                         rdfs:comment "A general comment can be made on the data source, assumptions and calculations for the production volume data." .


###  http://www.EcoInvent.org/EcoSpold02/flowdata#productionVolumeMathematicalRelation
:productionVolumeMathematicalRelation rdf:type owl:DatatypeProperty ;
                                      rdfs:domain :TIntermediateExchange ;
                                      rdfs:range xsd:string ;
                                      rdfs:comment """Defines a mathematical formula which references to values of flows, parameters or properties by variable names or REF function.
						The result of the formula with a specific set of variable values is written into the amount field.""" .


###  http://www.EcoInvent.org/EcoSpold02/flowdata#productionVolumeSourceContextId
:productionVolumeSourceContextId rdf:type owl:DatatypeProperty ;
                                 rdfs:domain :TIntermediateExchange ;
                                 rdfs:range xsd:string ;
                                 rdfs:comment """Reference to the context of the source.
						If this attribute is omitted the context of the dataset itself will be used instead.""" .


###  http://www.EcoInvent.org/EcoSpold02/flowdata#productionVolumeSourceFirstAuthor
:productionVolumeSourceFirstAuthor rdf:type owl:DatatypeProperty ;
                                   rdfs:domain :TIntermediateExchange ;
                                   rdfs:range xsd:string ;
                                   rdfs:comment "Indicates the first author by surname and abbreviated name (e.g., Einstein A.). In case of measurement on site, oral communication, personal written communication and questionnaries ('sourceType'=4, 5, 6, 7) the name of the communicating person is mentioned here." .


###  http://www.EcoInvent.org/EcoSpold02/flowdata#productionVolumeSourceId
:productionVolumeSourceId rdf:type owl:DatatypeProperty ;
                          rdfs:domain :TIntermediateExchange ;
                          rdfs:range xsd:string ;
                          rdfs:comment "A reference to a valid source." .


###  http://www.EcoInvent.org/EcoSpold02/flowdata#productionVolumeSourceIdOverwrittenByChild
:productionVolumeSourceIdOverwrittenByChild rdf:type owl:DatatypeProperty ;
                                            rdfs:domain :TIntermediateExchange ;
                                            rdfs:range xsd:string ;
                                            rdfs:comment "If a reference to a master data entity must be removed in a child dataset it is required to set the corresponding xxxOverwrittenByChild attribute to true. Otherwise the removed referenced will be interpreted as \"Keep the Parent Value\"." .


###  http://www.EcoInvent.org/EcoSpold02/flowdata#productionVolumeSourceYear
:productionVolumeSourceYear rdf:type owl:DatatypeProperty ;
                            rdfs:domain :TIntermediateExchange ;
                            rdfs:range xsd:string ;
                            rdfs:comment "Indicates the year of publication and communication, respectively. For web-sites: last visited." .


###  http://www.EcoInvent.org/EcoSpold02/flowdata#productionVolumeVariableName
:productionVolumeVariableName rdf:type owl:DatatypeProperty ;
                              rdfs:domain :TIntermediateExchange ;
                              rdfs:range xsd:string ;
                              rdfs:comment "The variable name is a short name for the production volume of the exchange, used when refering to the production volume amount in mathematical relations (formulas). Variables may contain characters, numbers and underscores (_). Variable names must start with a character (a-z). Variable names are not case sensitive (calorific_Value equals Calorific_value)." .


###  http://www.EcoInvent.org/EcoSpold02/flowdata#sourceContextId
:sourceContextId rdf:type owl:DatatypeProperty ;
                 rdfs:domain :TElementaryExchange ,
                             :TTransferCoefficient ;
                 rdfs:range xsd:string ;
                 rdfs:comment """Reference to the context of the source.
If this attribute is omitted the context of the dataset itself will be used instead.""" .


###  http://www.EcoInvent.org/EcoSpold02/flowdata#sourceFirstAuthor
:sourceFirstAuthor rdf:type owl:DatatypeProperty ;
                   rdfs:domain :TElementaryExchange ,
                               :TTransferCoefficient ;
                   rdfs:range xsd:string ;
                   rdfs:comment "Indicates the first author by surname and abbreviated name (e.g., Einstein A.). In case of measurement on site, oral communication, personal written communication and questionnaries ('sourceType'=4, 5, 6, 7) the name of the communicating person is mentioned here." .


###  http://www.EcoInvent.org/EcoSpold02/flowdata#sourceId
:sourceId rdf:type owl:DatatypeProperty ;
          rdfs:domain :TElementaryExchange ,
                      :TTransferCoefficient ;
          rdfs:range xsd:string ;
          rdfs:comment "Reference to a source defined in the modelling and validation section." .


###  http://www.EcoInvent.org/EcoSpold02/flowdata#sourceIdOverwrittenByChild
:sourceIdOverwrittenByChild rdf:type owl:DatatypeProperty ;
                            rdfs:domain :TElementaryExchange ,
                                        :TTransferCoefficient ;
                            rdfs:range xsd:string ;
                            rdfs:comment "If a reference to a master data entity must be removed in a child dataset it is required to set the corresponding xxxOverwrittenByChild attribute to true. Otherwise the removed referenced will be interpreted as \"Keep the Parent Value\"." .


###  http://www.EcoInvent.org/EcoSpold02/flowdata#sourceYear
:sourceYear rdf:type owl:DatatypeProperty ;
            rdfs:domain :TElementaryExchange ,
                        :TTransferCoefficient ;
            rdfs:range xsd:string ;
            rdfs:comment "Indicates the year of publication and communication, respectively. For web-sites: last visited." .


###  http://www.EcoInvent.org/EcoSpold02/flowdata#specificAllocationPropertyContextId
:specificAllocationPropertyContextId rdf:type owl:DatatypeProperty ;
                                     rdfs:domain :TElementaryExchange ;
                                     rdfs:range xsd:string ;
                                     rdfs:comment """Reference to the context of the property.
If this attribute is omitted the context of the dataset itself will be used instead.""" .


###  http://www.EcoInvent.org/EcoSpold02/flowdata#specificAllocationPropertyId
:specificAllocationPropertyId rdf:type owl:DatatypeProperty ;
                              rdfs:domain :TElementaryExchange ;
                              rdfs:range xsd:string ;
                              rdfs:comment "Reference to the Property used by the allocation. This overrides the dataset wide default defined by masterAllocationPropertyId." .


###  http://www.EcoInvent.org/EcoSpold02/flowdata#specificAllocationPropertyIdOverwrittenByChild
:specificAllocationPropertyIdOverwrittenByChild rdf:type owl:DatatypeProperty ;
                                                rdfs:domain :TElementaryExchange ;
                                                rdfs:range xsd:string ;
                                                rdfs:comment "If a reference to a master data entity must be removed in a child dataset it is required to set the corresponding xxxOverwrittenByChild attribute to true. Otherwise the removed referenced will be interpreted as \"Keep the Parent Value\"." .


###  http://www.EcoInvent.org/EcoSpold02/flowdata#synonym
:synonym rdf:type owl:DatatypeProperty ;
         rdfs:domain :TCustomExchange ;
         rdfs:range xsd:string ;
         rdfs:comment """List of synonyms for the name. Contrary to normal multi language strings, synonyms may contain more than one element with the same xml:lang attribute value.
0..n entries are allowed with a max. length of 80 each.""" .


###  http://www.EcoInvent.org/EcoSpold02/flowdata#tag
:tag rdf:type owl:DatatypeProperty ;
     rdfs:domain :TCustomExchange ;
     rdfs:range xsd:string ;
     rdfs:comment "The tag field allows an open list of keywords which describes the activity and can be used for filtering, grouping and searching. The validTags file reference provides a list of predefined tags, but the semantic validation procedure should only display an information (not an error) if a tag entry cannot be found in the validTags master file." .


###  http://www.EcoInvent.org/EcoSpold02/flowdata#unitContextId
:unitContextId rdf:type owl:DatatypeProperty ;
               rdfs:domain :TElementaryExchange ,
                           :TParameter ;
               rdfs:range xsd:string ;
               rdfs:comment """Reference to the context of the unit.
If this attribute is omitted the context of the dataset itself will be used instead.""" .


###  http://www.EcoInvent.org/EcoSpold02/flowdata#unitId
:unitId rdf:type owl:DatatypeProperty ;
        rdfs:domain :TCustomExchange ;
        rdfs:range xsd:string ;
        rdfs:comment "Reference to the unit of the parameter amount." .


###  http://www.EcoInvent.org/EcoSpold02/flowdata#unitName
:unitName rdf:type owl:DatatypeProperty ;
          rdfs:domain :TCustomExchange ,
                      :TElementaryExchange ,
                      :TImpactIndicatorResult ,
                      :TParameter ;
          rdfs:range xsd:string ;
          rdfs:comment "Unit name of the amount." .


###  http://www.EcoInvent.org/EcoSpold02/flowdata#variableName
:variableName rdf:type owl:DatatypeProperty ;
              rdfs:domain :TElementaryExchange ,
                          :TParameter ;
              rdfs:range xsd:string ;
              rdfs:comment "The variable name is a short name for the exchange, used when refering to the exchange amount in mathematical relations (formulas). Variables may contain characters, numbers and underscores (_). Variable names must start with a character (a-z). Variable names are not case sensitive (calorific_Value equals Calorific_value)." .


###  http://www.EcoInvent.org/EcoSpold02/metainformation#comment
<http://www.EcoInvent.org/EcoSpold02/metainformation#comment> rdf:type owl:DatatypeProperty .


###  http://www.EcoInvent.org/EcoSpold02/metainformation#id
<http://www.EcoInvent.org/EcoSpold02/metainformation#id> rdf:type owl:DatatypeProperty .


#################################################################
#    Classes
#################################################################

###  http://www.EcoInvent.org/EcoSpold02/flowdata#TCustomExchange
:TCustomExchange rdf:type owl:Class ;
                 rdfs:subClassOf [ rdf:type owl:Restriction ;
                                   owl:onProperty :transferCoefficient ;
                                   owl:someValuesFrom :TTransferCoefficient
                                 ] ,
                                 [ rdf:type owl:Restriction ;
                                   owl:onProperty :name ;
                                   owl:maxQualifiedCardinality "1"^^xsd:nonNegativeInteger ;
                                   owl:onDataRange xsd:string
                                 ] ,
                                 [ rdf:type owl:Restriction ;
                                   owl:onProperty :synonym ;
                                   owl:maxQualifiedCardinality "1"^^xsd:nonNegativeInteger ;
                                   owl:onDataRange xsd:string
                                 ] ,
                                 [ rdf:type owl:Restriction ;
                                   owl:onProperty :tag ;
                                   owl:maxQualifiedCardinality "1"^^xsd:nonNegativeInteger ;
                                   owl:onDataRange xsd:string
                                 ] ,
                                 [ rdf:type owl:Restriction ;
                                   owl:onProperty :unitName ;
                                   owl:maxQualifiedCardinality "1"^^xsd:nonNegativeInteger ;
                                   owl:onDataRange xsd:string
                                 ] ;
                 rdfs:comment "This section contains elements used in both exchange types. Elements unique to either Intermediate exchanges or Exchanges with environment are listed in the sections below." .


###  http://www.EcoInvent.org/EcoSpold02/flowdata#TElementaryExchange
:TElementaryExchange rdf:type owl:Class ;
                     rdfs:subClassOf :TCustomExchange ,
                                     [ rdf:type owl:Restriction ;
                                       owl:onProperty :amount ;
                                       owl:maxQualifiedCardinality "1"^^xsd:nonNegativeInteger ;
                                       owl:onDataRange xsd:float
                                     ] ,
                                     [ rdf:type owl:Restriction ;
                                       owl:onProperty :casNumber ;
                                       owl:maxQualifiedCardinality "1"^^xsd:nonNegativeInteger ;
                                       owl:onDataRange xsd:string
                                     ] ,
                                     [ rdf:type owl:Restriction ;
                                       owl:onProperty :elementaryExchangeContextId ;
                                       owl:maxQualifiedCardinality "1"^^xsd:nonNegativeInteger ;
                                       owl:onDataRange xsd:string
                                     ] ,
                                     [ rdf:type owl:Restriction ;
                                       owl:onProperty :elementaryExchangeId ;
                                       owl:maxQualifiedCardinality "1"^^xsd:nonNegativeInteger ;
                                       owl:onDataRange xsd:string
                                     ] ,
                                     [ rdf:type owl:Restriction ;
                                       owl:onProperty :exchangeId ;
                                       owl:maxQualifiedCardinality "1"^^xsd:nonNegativeInteger ;
                                       owl:onDataRange xsd:string
                                     ] ,
                                     [ rdf:type owl:Restriction ;
                                       owl:onProperty :formula ;
                                       owl:maxQualifiedCardinality "1"^^xsd:nonNegativeInteger ;
                                       owl:onDataRange xsd:string
                                     ] ,
                                     [ rdf:type owl:Restriction ;
                                       owl:onProperty :isCalculatedAmount ;
                                       owl:maxQualifiedCardinality "1"^^xsd:nonNegativeInteger ;
                                       owl:onDataRange xsd:boolean
                                     ] ,
                                     [ rdf:type owl:Restriction ;
                                       owl:onProperty :mathematicalRelation ;
                                       owl:maxQualifiedCardinality "1"^^xsd:nonNegativeInteger ;
                                       owl:onDataRange xsd:string
                                     ] ,
                                     [ rdf:type owl:Restriction ;
                                       owl:onProperty :name ;
                                       owl:maxQualifiedCardinality "1"^^xsd:nonNegativeInteger ;
                                       owl:onDataRange xsd:string
                                     ] ,
                                     [ rdf:type owl:Restriction ;
                                       owl:onProperty :pageNumbers ;
                                       owl:maxQualifiedCardinality "1"^^xsd:nonNegativeInteger ;
                                       owl:onDataRange xsd:string
                                     ] ,
                                     [ rdf:type owl:Restriction ;
                                       owl:onProperty :sourceContextId ;
                                       owl:maxQualifiedCardinality "1"^^xsd:nonNegativeInteger ;
                                       owl:onDataRange xsd:string
                                     ] ,
                                     [ rdf:type owl:Restriction ;
                                       owl:onProperty :sourceFirstAuthor ;
                                       owl:maxQualifiedCardinality "1"^^xsd:nonNegativeInteger ;
                                       owl:onDataRange xsd:string
                                     ] ,
                                     [ rdf:type owl:Restriction ;
                                       owl:onProperty :sourceId ;
                                       owl:maxQualifiedCardinality "1"^^xsd:nonNegativeInteger ;
                                       owl:onDataRange xsd:string
                                     ] ,
                                     [ rdf:type owl:Restriction ;
                                       owl:onProperty :sourceIdOverwrittenByChild ;
                                       owl:maxQualifiedCardinality "1"^^xsd:nonNegativeInteger ;
                                       owl:onDataRange xsd:string
                                     ] ,
                                     [ rdf:type owl:Restriction ;
                                       owl:onProperty :sourceYear ;
                                       owl:maxQualifiedCardinality "1"^^xsd:nonNegativeInteger ;
                                       owl:onDataRange xsd:string
                                     ] ,
                                     [ rdf:type owl:Restriction ;
                                       owl:onProperty :specificAllocationPropertyContextId ;
                                       owl:maxQualifiedCardinality "1"^^xsd:nonNegativeInteger ;
                                       owl:onDataRange xsd:string
                                     ] ,
                                     [ rdf:type owl:Restriction ;
                                       owl:onProperty :specificAllocationPropertyId ;
                                       owl:maxQualifiedCardinality "1"^^xsd:nonNegativeInteger ;
                                       owl:onDataRange xsd:string
                                     ] ,
                                     [ rdf:type owl:Restriction ;
                                       owl:onProperty :specificAllocationPropertyIdOverwrittenByChild ;
                                       owl:maxQualifiedCardinality "1"^^xsd:nonNegativeInteger ;
                                       owl:onDataRange xsd:boolean
                                     ] ,
                                     [ rdf:type owl:Restriction ;
                                       owl:onProperty :unitContextId ;
                                       owl:maxQualifiedCardinality "1"^^xsd:nonNegativeInteger ;
                                       owl:onDataRange xsd:string
                                     ] ,
                                     [ rdf:type owl:Restriction ;
                                       owl:onProperty :unitName ;
                                       owl:maxQualifiedCardinality "1"^^xsd:nonNegativeInteger ;
                                       owl:onDataRange xsd:string
                                     ] ,
                                     [ rdf:type owl:Restriction ;
                                       owl:onProperty :variableName ;
                                       owl:maxQualifiedCardinality "1"^^xsd:nonNegativeInteger ;
                                       owl:onDataRange xsd:string
                                     ] ,
                                     [ rdf:type owl:Restriction ;
                                       owl:onProperty <http://www.EcoInvent.org/EcoSpold02/metainformation#id> ;
                                       owl:maxQualifiedCardinality "1"^^xsd:nonNegativeInteger ;
                                       owl:onDataRange xsd:string
                                     ] ;
                     rdfs:comment """Comprises fields (additional to the exchanges section) which are only valid for elementary exchanges. Exchanges with environment are elementary flows as inputs and outputs recorded in a unit process and its related information.

This section extends the exchanges section in case of exchanges with environment.""" .


###  http://www.EcoInvent.org/EcoSpold02/flowdata#TImpactIndicatorResult
:TImpactIndicatorResult rdf:type owl:Class ;
                        rdfs:subClassOf [ rdf:type owl:Restriction ;
                                          owl:onProperty :amount ;
                                          owl:maxQualifiedCardinality "1"^^xsd:nonNegativeInteger ;
                                          owl:onDataRange xsd:float
                                        ] ,
                                        [ rdf:type owl:Restriction ;
                                          owl:onProperty :impactCategoryContextId ;
                                          owl:maxQualifiedCardinality "1"^^xsd:nonNegativeInteger ;
                                          owl:onDataRange xsd:string
                                        ] ,
                                        [ rdf:type owl:Restriction ;
                                          owl:onProperty :impactCategoryId ;
                                          owl:maxQualifiedCardinality "1"^^xsd:nonNegativeInteger ;
                                          owl:onDataRange xsd:string
                                        ] ,
                                        [ rdf:type owl:Restriction ;
                                          owl:onProperty :impactCategoryName ;
                                          owl:maxQualifiedCardinality "1"^^xsd:nonNegativeInteger ;
                                          owl:onDataRange xsd:string
                                        ] ,
                                        [ rdf:type owl:Restriction ;
                                          owl:onProperty :impactIndicatorContextId ;
                                          owl:maxQualifiedCardinality "1"^^xsd:nonNegativeInteger ;
                                          owl:onDataRange xsd:string
                                        ] ,
                                        [ rdf:type owl:Restriction ;
                                          owl:onProperty :impactIndicatorId ;
                                          owl:maxQualifiedCardinality "1"^^xsd:nonNegativeInteger ;
                                          owl:onDataRange xsd:string
                                        ] ,
                                        [ rdf:type owl:Restriction ;
                                          owl:onProperty :impactMethodContextId ;
                                          owl:maxQualifiedCardinality "1"^^xsd:nonNegativeInteger ;
                                          owl:onDataRange xsd:string
                                        ] ,
                                        [ rdf:type owl:Restriction ;
                                          owl:onProperty :impactMethodId ;
                                          owl:maxQualifiedCardinality "1"^^xsd:nonNegativeInteger ;
                                          owl:onDataRange xsd:string
                                        ] ,
                                        [ rdf:type owl:Restriction ;
                                          owl:onProperty :impactMethodName ;
                                          owl:maxQualifiedCardinality "1"^^xsd:nonNegativeInteger ;
                                          owl:onDataRange xsd:string
                                        ] ,
                                        [ rdf:type owl:Restriction ;
                                          owl:onProperty :name ;
                                          owl:maxQualifiedCardinality "1"^^xsd:nonNegativeInteger ;
                                          owl:onDataRange xsd:string
                                        ] ,
                                        [ rdf:type owl:Restriction ;
                                          owl:onProperty :unitName ;
                                          owl:maxQualifiedCardinality "1"^^xsd:nonNegativeInteger ;
                                          owl:onDataRange xsd:string
                                        ] ;
                        rdfs:comment "Calculated impact indicators" .


###  http://www.EcoInvent.org/EcoSpold02/flowdata#TIntermediateExchange
:TIntermediateExchange rdf:type owl:Class ;
                       rdfs:subClassOf :TCustomExchange ,
                                       [ rdf:type owl:Restriction ;
                                         owl:onProperty :activityLinkContextId ;
                                         owl:maxQualifiedCardinality "1"^^xsd:nonNegativeInteger ;
                                         owl:onDataRange xsd:string
                                       ] ,
                                       [ rdf:type owl:Restriction ;
                                         owl:onProperty :activityLinkId ;
                                         owl:maxQualifiedCardinality "1"^^xsd:nonNegativeInteger ;
                                         owl:onDataRange xsd:string
                                       ] ,
                                       [ rdf:type owl:Restriction ;
                                         owl:onProperty :activityLinkIdOverwrittenByChild ;
                                         owl:maxQualifiedCardinality "1"^^xsd:nonNegativeInteger ;
                                         owl:onDataRange xsd:string
                                       ] ,
                                       [ rdf:type owl:Restriction ;
                                         owl:onProperty :intermediateExchangeContextId ;
                                         owl:maxQualifiedCardinality "1"^^xsd:nonNegativeInteger ;
                                         owl:onDataRange xsd:string
                                       ] ,
                                       [ rdf:type owl:Restriction ;
                                         owl:onProperty :intermediateExchangeId ;
                                         owl:maxQualifiedCardinality "1"^^xsd:nonNegativeInteger ;
                                         owl:onDataRange xsd:string
                                       ] ,
                                       [ rdf:type owl:Restriction ;
                                         owl:onProperty :productionVolumeAmount ;
                                         owl:maxQualifiedCardinality "1"^^xsd:nonNegativeInteger ;
                                         owl:onDataRange xsd:float
                                       ] ,
                                       [ rdf:type owl:Restriction ;
                                         owl:onProperty :productionVolumeComment ;
                                         owl:maxQualifiedCardinality "1"^^xsd:nonNegativeInteger ;
                                         owl:onDataRange xsd:string
                                       ] ,
                                       [ rdf:type owl:Restriction ;
                                         owl:onProperty :productionVolumeMathematicalRelation ;
                                         owl:maxQualifiedCardinality "1"^^xsd:nonNegativeInteger ;
                                         owl:onDataRange xsd:string
                                       ] ,
                                       [ rdf:type owl:Restriction ;
                                         owl:onProperty :productionVolumeSourceContextId ;
                                         owl:maxQualifiedCardinality "1"^^xsd:nonNegativeInteger ;
                                         owl:onDataRange xsd:string
                                       ] ,
                                       [ rdf:type owl:Restriction ;
                                         owl:onProperty :productionVolumeSourceFirstAuthor ;
                                         owl:maxQualifiedCardinality "1"^^xsd:nonNegativeInteger ;
                                         owl:onDataRange xsd:string
                                       ] ,
                                       [ rdf:type owl:Restriction ;
                                         owl:onProperty :productionVolumeSourceId ;
                                         owl:maxQualifiedCardinality "1"^^xsd:nonNegativeInteger ;
                                         owl:onDataRange xsd:string
                                       ] ,
                                       [ rdf:type owl:Restriction ;
                                         owl:onProperty :productionVolumeSourceIdOverwrittenByChild ;
                                         owl:maxQualifiedCardinality "1"^^xsd:nonNegativeInteger ;
                                         owl:onDataRange xsd:string
                                       ] ,
                                       [ rdf:type owl:Restriction ;
                                         owl:onProperty :productionVolumeSourceYear ;
                                         owl:maxQualifiedCardinality "1"^^xsd:nonNegativeInteger ;
                                         owl:onDataRange xsd:string
                                       ] ,
                                       [ rdf:type owl:Restriction ;
                                         owl:onProperty :productionVolumeVariableName ;
                                         owl:maxQualifiedCardinality "1"^^xsd:nonNegativeInteger ;
                                         owl:onDataRange xsd:string
                                       ] ;
                       rdfs:comment """Comprises fields (additional to the exchanges section) which are only valid for intermediate exchanges. Intermediate exchanges are 
product or waste inputs and outputs recorded in a unit process and its related information.

This section extends the exchanges section in case of intermediate exchanges.""" .


###  http://www.EcoInvent.org/EcoSpold02/flowdata#TParameter
:TParameter rdf:type owl:Class ;
            rdfs:subClassOf [ rdf:type owl:Restriction ;
                              owl:onProperty :amount ;
                              owl:maxQualifiedCardinality "1"^^xsd:nonNegativeInteger ;
                              owl:onDataRange xsd:float
                            ] ,
                            [ rdf:type owl:Restriction ;
                              owl:onProperty :isCalculatedAmount ;
                              owl:maxQualifiedCardinality "1"^^xsd:nonNegativeInteger ;
                              owl:onDataRange xsd:boolean
                            ] ,
                            [ rdf:type owl:Restriction ;
                              owl:onProperty :mathematicalRelation ;
                              owl:maxQualifiedCardinality "1"^^xsd:nonNegativeInteger ;
                              owl:onDataRange xsd:string
                            ] ,
                            [ rdf:type owl:Restriction ;
                              owl:onProperty :name ;
                              owl:maxQualifiedCardinality "1"^^xsd:nonNegativeInteger ;
                              owl:onDataRange xsd:string
                            ] ,
                            [ rdf:type owl:Restriction ;
                              owl:onProperty :parameterContextId ;
                              owl:maxQualifiedCardinality "1"^^xsd:nonNegativeInteger ;
                              owl:onDataRange xsd:string
                            ] ,
                            [ rdf:type owl:Restriction ;
                              owl:onProperty :parameterId ;
                              owl:maxQualifiedCardinality "1"^^xsd:nonNegativeInteger ;
                              owl:onDataRange xsd:string
                            ] ,
                            [ rdf:type owl:Restriction ;
                              owl:onProperty :unitContextId ;
                              owl:maxQualifiedCardinality "1"^^xsd:nonNegativeInteger ;
                              owl:onDataRange xsd:string
                            ] ,
                            [ rdf:type owl:Restriction ;
                              owl:onProperty :unitId ;
                              owl:maxQualifiedCardinality "1"^^xsd:nonNegativeInteger ;
                              owl:onDataRange xsd:string
                            ] ,
                            [ rdf:type owl:Restriction ;
                              owl:onProperty :unitName ;
                              owl:maxQualifiedCardinality "1"^^xsd:nonNegativeInteger ;
                              owl:onDataRange xsd:string
                            ] ,
                            [ rdf:type owl:Restriction ;
                              owl:onProperty :variableName ;
                              owl:maxQualifiedCardinality "1"^^xsd:nonNegativeInteger ;
                              owl:onDataRange xsd:string
                            ] ,
                            [ rdf:type owl:Restriction ;
                              owl:onProperty <http://www.EcoInvent.org/EcoSpold02/metainformation#comment> ;
                              owl:maxQualifiedCardinality "1"^^xsd:nonNegativeInteger ;
                              owl:onDataRange xsd:string
                            ] .


###  http://www.EcoInvent.org/EcoSpold02/flowdata#TTransferCoefficient
:TTransferCoefficient rdf:type owl:Class ;
                      rdfs:subClassOf [ rdf:type owl:Restriction ;
                                        owl:onProperty :amount ;
                                        owl:maxQualifiedCardinality "1"^^xsd:nonNegativeInteger ;
                                        owl:onDataRange xsd:float
                                      ] ,
                                      [ rdf:type owl:Restriction ;
                                        owl:onProperty :exchangeId ;
                                        owl:maxQualifiedCardinality "1"^^xsd:nonNegativeInteger ;
                                        owl:onDataRange xsd:string
                                      ] ,
                                      [ rdf:type owl:Restriction ;
                                        owl:onProperty :isCalculatedAmount ;
                                        owl:maxQualifiedCardinality "1"^^xsd:nonNegativeInteger ;
                                        owl:onDataRange xsd:boolean
                                      ] ,
                                      [ rdf:type owl:Restriction ;
                                        owl:onProperty :mathematicalRelation ;
                                        owl:maxQualifiedCardinality "1"^^xsd:nonNegativeInteger ;
                                        owl:onDataRange xsd:string
                                      ] ,
                                      [ rdf:type owl:Restriction ;
                                        owl:onProperty :sourceContextId ;
                                        owl:maxQualifiedCardinality "1"^^xsd:nonNegativeInteger ;
                                        owl:onDataRange xsd:string
                                      ] ,
                                      [ rdf:type owl:Restriction ;
                                        owl:onProperty :sourceFirstAuthor ;
                                        owl:maxQualifiedCardinality "1"^^xsd:nonNegativeInteger ;
                                        owl:onDataRange xsd:string
                                      ] ,
                                      [ rdf:type owl:Restriction ;
                                        owl:onProperty :sourceId ;
                                        owl:maxQualifiedCardinality "1"^^xsd:nonNegativeInteger ;
                                        owl:onDataRange xsd:string
                                      ] ,
                                      [ rdf:type owl:Restriction ;
                                        owl:onProperty :sourceIdOverwrittenByChild ;
                                        owl:maxQualifiedCardinality "1"^^xsd:nonNegativeInteger ;
                                        owl:onDataRange xsd:boolean
                                      ] ,
                                      [ rdf:type owl:Restriction ;
                                        owl:onProperty :sourceYear ;
                                        owl:maxQualifiedCardinality "1"^^xsd:nonNegativeInteger ;
                                        owl:onDataRange xsd:string
                                      ] ,
                                      [ rdf:type owl:Restriction ;
                                        owl:onProperty <http://www.EcoInvent.org/EcoSpold02/metainformation#comment> ;
                                        owl:maxQualifiedCardinality "1"^^xsd:nonNegativeInteger ;
                                        owl:onDataRange xsd:string
                                      ] ;
                      rdfs:comment "Transfer coefficients for calculating amounts of outputs from amounts of inputs." .


[ xsd:minInclusive 1
] .

[ owl:maxCardinality "1"^^xsd:int
 ] .

[ xsd:minInclusive 4
 ] .

[ owl:maxCardinality "1"^^xsd:int
 ] .

[ xsd:maxInclusive 5
 ] .

[ owl:maxCardinality "1"^^xsd:int
 ] .

[ xsd:minInclusive 1
 ] .

[ owl:maxCardinality "1"^^xsd:int
 ] .

[ owl:maxCardinality "1"^^xsd:int
 ] .

[ xsd:maxInclusive 4
 ] .

[ xsd:minInclusive 1
 ] .

[ owl:maxCardinality "1"^^xsd:int
 ] .

[ owl:maxCardinality "1"^^xsd:int
 ] .

[ xsd:minInclusive 1
 ] .

[ owl:maxCardinality "1"^^xsd:int
 ] .

[ xsd:maxInclusive 5
 ] .

[ xsd:minInclusive 1
 ] .

[ owl:maxCardinality "1"^^xsd:int
 ] .

[ owl:maxCardinality "1"^^xsd:int
 ] .

[ xsd:maxInclusive 5
 ] .

[ xsd:maxInclusive 5
 ] .

[ owl:maxCardinality "1"^^xsd:int
 ] .

[ xsd:maxInclusive 5
 ] .

[ owl:maxCardinality "1"^^xsd:int
 ] .

[ owl:maxCardinality "1"^^xsd:int
 ] .

###  Generated by the OWL API (version 4.5.9.2019-02-01T07:24:44Z) https://github.com/owlcs/owlapi
